finish proof of jordan hoelder

src/jordan_hoelder.lean
@@ -11,54 +11,65 @@ universe u
 
 open set
 
-class jordan_hoelder_class (X : Type u) extends bounded_lattice X :=
+class jordan_hoelder_class (X : Type u) [lattice X] :=
 (is_maximal : X → X → Prop)
-(lt_of_is_maximal : ∀ x y, is_maximal x y → x < y)
+(lt_of_is_maximal : ∀ {x y}, is_maximal x y → x < y)
 (isom : (X × X) → (X × X) → Prop)
+(isom_refl : ∀ x, isom x x)
+(isom_symm : ∀ {x y}, isom x y → isom y x)
+(isom_trans : ∀ {x y z}, isom x y → isom y z → isom x z)
+(second_iso : ∀ x y, isom (y, x ⊔ y) (x ⊓ y, x))
+(sup_eq_of_is_maximal : ∀ {x y z}, is_maximal x z → is_maximal y z →
+  x ≠ y → x ⊔ y = z)
+(is_maximal_inter : ∀ {x y z}, is_maximal x z → is_maximal y z → x ≠ y →
+  is_maximal (x ⊓ y) y)
 
-variables {X : Type u} [bounded_lattice X]
+open jordan_hoelder_class
 
-structure composition_series (is_maximal : X → X → Prop) : Type u :=
+attribute [refl] isom_refl
+attribute [symm] isom_symm
+attribute [trans] isom_trans
+
+structure composition_series (X : Type u) [lattice X] [jordan_hoelder_class X] : Type u :=
 (length : ℕ)
 (series : fin length.succ → X)
 (step' : ∀ i : fin length, is_maximal (series i.cast_succ) (series i.succ))
 
 namespace composition_series
 
-variable {im : X → X → Prop}
+variables {X : Type u} [lattice X] [jordan_hoelder_class X]
 
-instance : has_coe_to_fun (composition_series im) :=
+instance : has_coe_to_fun (composition_series X) :=
 { F := _, coe := composition_series.series }
 
 variables {X}
 
-lemma step (s : composition_series im) : ∀ i : fin s.length,
-  im (s i.cast_succ) (s i.succ) := s.step'
+lemma step (s : composition_series X) : ∀ i : fin s.length,
+  is_maximal (s i.cast_succ) (s i.succ) := s.step'
 
 @[simp] lemma coe_fn_mk (length : ℕ) (series step) :
-  (@composition_series.mk X _ im length series step : fin length.succ → X) = series := rfl
+  (@composition_series.mk X _ _ length series step : fin length.succ → X) = series := rfl
 
-theorem lt_succ (him : ∀ x y, im x y → x < y)(s : composition_series im) (i : fin s.length) :
+theorem lt_succ (s : composition_series X) (i : fin s.length) :
   s i.cast_succ < s i.succ :=
-him _ _ (s.step _)
+lt_of_is_maximal (s.step _)
 
-protected theorem strict_mono (s : composition_series im)
-  (him : ∀ x y, im x y → x < y) : strict_mono s :=
-fin.strict_mono_iff_lt_succ.2 (λ i h, s.lt_succ him ⟨i, nat.lt_of_succ_lt_succ h⟩)
+protected theorem strict_mono (s : composition_series X) : strict_mono s :=
+fin.strict_mono_iff_lt_succ.2 (λ i h, s.lt_succ ⟨i, nat.lt_of_succ_lt_succ h⟩)
 
-protected theorem injective (s : composition_series im) : function.injective s :=
+protected theorem injective (s : composition_series X) : function.injective s :=
 s.strict_mono.injective
 
-@[simp] protected theorem inj (s : composition_series im) {i j : fin s.length.succ} :
+@[simp] protected theorem inj (s : composition_series X) {i j : fin s.length.succ} :
   s i = s j ↔ i = j :=
 s.injective.eq_iff
 
-instance : has_mem X (composition_series im) :=
+instance : has_mem X (composition_series X) :=
 ⟨λ x s, x ∈ set.range s⟩
 
-lemma mem_def {x : X} {s : composition_series im} : x ∈ s ↔ x ∈ set.range s := iff.rfl
+lemma mem_def {x : X} {s : composition_series X} : x ∈ s ↔ x ∈ set.range s := iff.rfl
 
-lemma total {s : composition_series im} {x y : X} (hx : x ∈ s) (hy : y ∈ s) : x ≤ y ∨ y ≤ x :=
+lemma total {s : composition_series X} {x y : X} (hx : x ∈ s) (hy : y ∈ s) : x ≤ y ∨ y ≤ x :=
 begin
   rcases set.mem_range.1 hx with ⟨i, rfl⟩,
   rcases set.mem_range.1 hy with ⟨j, rfl⟩,
@@ -66,9 +77,9 @@ begin
   exact le_total i j
 end
 
-def to_list (s : composition_series im) : list X := list.of_fn s
+def to_list (s : composition_series X) : list X := list.of_fn s
 
-lemma ext_fun {s₁ s₂ : composition_series im}
+lemma ext_fun {s₁ s₂ : composition_series X}
   (hl : s₁.length = s₂.length)
   (h : ∀ i, s₁ i = s₂ (fin.cast (congr_arg nat.succ hl) i)) :
   s₁ = s₂ :=
@@ -79,10 +90,10 @@ begin
   simpa [function.funext_iff] using h
 end
 
-lemma length_to_list (s : composition_series im) : s.to_list.length = s.length.succ :=
+lemma length_to_list (s : composition_series X) : s.to_list.length = s.length.succ :=
 by rw [to_list, list.length_of_fn]
 
-lemma to_list_injective : function.injective (@composition_series.to_list X _) :=
+lemma to_list_injective : function.injective (@composition_series.to_list X _ _) :=
 λ s₁ s₂ (h : list.of_fn s₁ = list.of_fn s₂),
 have h₁ : s₁.length = s₂.length,
   from nat.succ_injective
@@ -104,7 +115,7 @@ begin
   exact funext h₂
 end
 
-lemma to_list_sorted (s : composition_series im) : s.to_list.sorted (<) :=
+lemma to_list_sorted (s : composition_series X) : s.to_list.sorted (<) :=
 list.pairwise_iff_nth_le.2 (λ i j hi hij,
   begin
     dsimp [to_list],
@@ -112,7 +123,7 @@ list.pairwise_iff_nth_le.2 (λ i j hi hij,
     exact s.strict_mono hij
   end)
 
-lemma to_list_nodup (s : composition_series im) : s.to_list.nodup :=
+lemma to_list_nodup (s : composition_series X) : s.to_list.nodup :=
 list.nodup_iff_nth_le_inj.2
   (λ i j hi hj,
     begin
@@ -121,13 +132,13 @@ list.nodup_iff_nth_le_inj.2
       exact id
     end)
 
-@[simp] lemma mem_to_list {s : composition_series im} {x : X} : x ∈ s.to_list ↔ x ∈ s :=
+@[simp] lemma mem_to_list {s : composition_series X} {x : X} : x ∈ s.to_list ↔ x ∈ s :=
 begin
   rw [to_list, list.mem_of_fn],
   refl
 end
 
-@[ext] lemma ext {s₁ s₂ : composition_series im} (h : ∀ x, x ∈ s₁ ↔ x ∈ s₂) : s₁ = s₂ :=
+@[ext] lemma ext {s₁ s₂ : composition_series X} (h : ∀ x, x ∈ s₁ ↔ x ∈ s₂) : s₁ = s₂ :=
 to_list_injective $ list.eq_of_perm_of_sorted
   (by classical; exact list.perm_of_nodup_nodup_to_finset_eq
     s₁.to_list_nodup
@@ -135,30 +146,30 @@ to_list_injective $ list.eq_of_perm_of_sorted
     (finset.ext $ by simp *))
   s₁.to_list_sorted s₂.to_list_sorted
 
-def top (s : composition_series im) : X := s (fin.last _)
+def top (s : composition_series X) : X := s (fin.last _)
 
-lemma top_mem (s : composition_series im) : s.top ∈ s :=
+lemma top_mem (s : composition_series X) : s.top ∈ s :=
 mem_def.2 (set.mem_range.2 ⟨fin.last _, rfl⟩)
 
-lemma le_top {s : composition_series im} {x : X} (hx : x ∈ s) : x ≤ s.top :=
+lemma le_top {s : composition_series X} {x : X} (hx : x ∈ s) : x ≤ s.top :=
 let ⟨i, hi⟩ := set.mem_range.1 hx in hi ▸ s.strict_mono.monotone (fin.le_last _)
 
-def bot (s : composition_series im) : X := s 0
+def bot (s : composition_series X) : X := s 0
 
-lemma bot_mem (s : composition_series im) : s.bot ∈ s :=
+lemma bot_mem (s : composition_series X) : s.bot ∈ s :=
 mem_def.2 (set.mem_range.2 ⟨0, rfl⟩)
 
-lemma bot_le {s : composition_series im} {x : X} (hx : x ∈ s) : s.bot ≤ x :=
+lemma bot_le {s : composition_series X} {x : X} (hx : x ∈ s) : s.bot ≤ x :=
 let ⟨i, hi⟩ := set.mem_range.1 hx in hi ▸ s.strict_mono.monotone (fin.zero_le _)
 
-instance : set_like (composition_series im) X :=
+instance : set_like (composition_series X) X :=
 { coe := λ s, set.range s,
   coe_injective' := λ s₁ s₂ h, ext $ λ x, begin
     dsimp at h,
     rw [mem_def, mem_def, h]
   end }
 
-@[simps] def erase_top (s : composition_series im) : composition_series im :=
+@[simps] def erase_top (s : composition_series X) : composition_series X :=
 { length := s.length - 1,
   series := λ i, s ⟨i, lt_of_lt_of_le i.2 (nat.succ_le_succ (nat.sub_le_self _ _))⟩,
   step' := λ i, begin
@@ -167,7 +178,7 @@ instance : set_like (composition_series im) X :=
     exact this
   end }
 
-lemma top_erase_top (s : composition_series im) :
+lemma top_erase_top (s : composition_series X) :
   s.erase_top.top = s ⟨s.length - 1, lt_of_le_of_lt (nat.sub_le_self _ _) (nat.lt_succ_self _)⟩ :=
 show s _ = s _, from congr_arg s
 begin
@@ -176,9 +187,9 @@ begin
     fin.coe_mk, coe_coe]
 end
 
-@[simp] lemma bot_erase_top (s : composition_series im) : s.erase_top.bot = s.bot := rfl
+@[simp] lemma bot_erase_top (s : composition_series X) : s.erase_top.bot = s.bot := rfl
 
-lemma length_pos_of_mem_ne {s : composition_series im}
+lemma length_pos_of_mem_ne {s : composition_series X}
   {x y : X} (hx : x ∈ s) (hy : y ∈ s) (hxy : x ≠ y) :
   0 < s.length :=
 let ⟨i, hi⟩ := hx, ⟨j, hj⟩ := hy in
@@ -189,7 +200,11 @@ hij.lt_or_lt.elim
   (λ hji, (lt_of_le_of_lt (zero_le j)
     (lt_of_lt_of_le hji (nat.le_of_lt_succ i.2))))
 
-lemma mem_erase_top_of_ne_of_mem {s : composition_series im} {x : X}
+lemma forall_mem_eq_of_length_eq_zero {s : composition_series X}
+  (hs : s.length = 0) {x y} (hx : x ∈ s) (hy : y ∈ s) : x = y :=
+by_contradiction (λ hxy, pos_iff_ne_zero.1 (length_pos_of_mem_ne hx hy hxy) hs)
+
+lemma mem_erase_top_of_ne_of_mem {s : composition_series X} {x : X}
   (hx : x ≠ s.top) (hxs : x ∈ s) : x ∈ s.erase_top :=
 begin
   { rcases hxs with ⟨i, rfl⟩,
@@ -203,13 +218,13 @@ begin
     simp [fin.ext_iff, nat.mod_eq_of_lt hi] }
 end
 
-lemma erase_top_le (s : composition_series im) : s.erase_top ≤ s :=
+lemma erase_top_le (s : composition_series X) : s.erase_top ≤ s :=
 begin
   rintros x ⟨i, rfl⟩,
   simp [mem_def],
 end
 
-lemma mem_erase_top {s : composition_series im} {x : X}
+lemma mem_erase_top {s : composition_series X} {x : X}
   (h : 0 < s.length) : x ∈ s.erase_top ↔ x ≠ s.top ∧ x ∈ s :=
 begin
   simp only [mem_def],
@@ -225,14 +240,19 @@ begin
 end
 
 lemma lt_top_of_mem_erase_top
-  {s : composition_series im} {x : X}
+  {s : composition_series X} {x : X}
   (h : 0 < s.length)
   (hx : x ∈ s.erase_top) :
   x < s.top :=
-lt_of_le_of_ne (le_top (s.erase_top_le hx)) ((mem_erase_top h).1 hx).1
+begin
+  rcases hx with ⟨⟨i, hi⟩, rfl⟩,
+  refine s.strict_mono _,
+  simp only [fin.lt_iff_coe_lt_coe, fin.coe_last, fin.coe_mk],
+  rwa [erase_top_length, nat.sub_succ, nat.sub_zero, nat.succ_pred_eq_of_pos h] at hi
+end
 
-lemma Ico_erase_top_top {s : composition_series im} (h : 0 < s.length) :
-  Ico s.erase_top.top s.top = {s.erase_top.top} :=
+lemma is_maximal_erase_top_top {s : composition_series X} (h : 0 < s.length) :
+  is_maximal s.erase_top.top s.top :=
 have s.length - 1 + 1 = s.length,
   by conv_rhs { rw [← nat.succ_sub_one s.length] }; rw nat.succ_sub h,
 begin
@@ -242,7 +262,7 @@ begin
 end
 
 lemma append_cast_add_aux
-  {s₁ s₂ : composition_series im}
+  {s₁ s₂ : composition_series X}
   (h : s₁ (fin.last _) = s₂ 0)
   (i : fin s₁.length) :
   fin.append (nat.add_succ _ _).symm (s₁ ∘ fin.cast_succ) s₂
@@ -250,7 +270,7 @@ lemma append_cast_add_aux
 by { cases i, simp [fin.append, *] }
 
 lemma append_succ_cast_add_aux
-  {s₁ s₂ : composition_series im}
+  {s₁ s₂ : composition_series X}
   (h : s₁ (fin.last _) = s₂ 0)
   (i : fin s₁.length) :
   fin.append (nat.add_succ _ _).symm (s₁ ∘ fin.cast_succ) s₂
@@ -269,7 +289,7 @@ begin
 end
 
 lemma append_cast_add_right_aux
-  {s₁ s₂ : composition_series im}
+  {s₁ s₂ : composition_series X}
   (h : s₁ (fin.last _) = s₂ 0)
   (i : fin s₂.length) :
   fin.append (nat.add_succ _ _).symm (s₁ ∘ fin.cast_succ) s₂
@@ -277,7 +297,7 @@ lemma append_cast_add_right_aux
 by { cases i, simp [fin.append, *] }
 
 lemma append_succ_cast_add_right_aux
-  {s₁ s₂ : composition_series im}
+  {s₁ s₂ : composition_series X}
   (h : s₁ (fin.last _) = s₂ 0)
   (i : fin s₂.length) :
   fin.append (nat.add_succ _ _).symm (s₁ ∘ fin.cast_succ) s₂
@@ -287,9 +307,9 @@ begin
   simp [fin.append, add_assoc]
 end
 
-@[simps length] def append {s₁ s₂ : composition_series im}
+@[simps length] def append {s₁ s₂ : composition_series X}
   (h : s₁.top = s₂.bot) :
-  composition_series im :=
+  composition_series X :=
 { length := s₁.length + s₂.length,
   series := fin.append (nat.add_succ _ _).symm (s₁ ∘ fin.cast_succ) s₂,
   step' := λ i, begin
@@ -303,87 +323,89 @@ end
   end }
 
 @[simp] lemma append_cast_add
-  {s₁ s₂ : composition_series im}
+  {s₁ s₂ : composition_series X}
   (h : s₁.top = s₂.bot)
   (i : fin s₁.length) :
   append h (fin.cast_add s₂.length i).cast_succ = s₁ i.cast_succ :=
 append_cast_add_aux h i
 
 @[simp] lemma append_succ_cast_add
-  {s₁ s₂ : composition_series im}
+  {s₁ s₂ : composition_series X}
   (h : s₁.top = s₂.bot)
   (i : fin s₁.length) :
   append h (fin.cast_add s₂.length i).succ = s₁ i.succ :=
 append_succ_cast_add_aux h i
 
 @[simp] lemma append_cast_add_right
-  {s₁ s₂ : composition_series im}
+  {s₁ s₂ : composition_series X}
   (h : s₁.top = s₂.bot)
   (i : fin s₂.length) :
   append h (fin.cast_add_right s₁.length i).cast_succ = s₂ i.cast_succ :=
 append_cast_add_right_aux h i
 
 @[simp] lemma append_succ_cast_add_right
-  {s₁ s₂ : composition_series im}
+  {s₁ s₂ : composition_series X}
   (h : s₁.top = s₂.bot)
   (i : fin s₂.length) :
   append h (fin.cast_add_right s₁.length i).succ = s₂ i.succ :=
 append_succ_cast_add_right_aux h i
 
 @[simps] def insert
-  (s : composition_series im)
+  (s : composition_series X)
   (x : X)
-  (hlt : ∀ y ∈ s, y < x)
-  (hsat : Ico s.top x = {s.top}) :
-  composition_series im :=
+  (hsat : is_maximal s.top x) :
+  composition_series X :=
 { length := s.length + 1,
   series := fin.snoc s x,
   step' := λ i, begin
     refine fin.last_cases _ _ i,
-    { rw [fin.snoc_cast_succ, fin.succ_last, fin.snoc_last, ← top, hsat] },
+    { rwa [fin.snoc_cast_succ, fin.succ_last, fin.snoc_last, ← top] },
     { intro i,
       rw [fin.snoc_cast_succ, ← fin.cast_succ_fin_succ, fin.snoc_cast_succ],
       exact s.step _ }
   end }
 
-@[simp] lemma insert_series'
-  (s : composition_series im)
-  (x : X)
-  (hlt : ∀ y ∈ s, y < x)
-  (hsat : Ico s.top x = {s.top}) :
-  @eq (fin (s.length + 2) → X) (insert s x hlt hsat) (fin.snoc s x) :=
-rfl
+-- @[simp] lemma insert_series'
+--   (s : composition_series X)
+--   (x : X)
+--   (hlt : ∀ y ∈ s, y < x)
+--   (hsat : is_maximal s.top x) :
+--   @eq (fin (s.length + 2) → X) (insert s x hlt hsat) (fin.snoc s x) :=
+-- rfl
 
 @[simp] lemma top_insert
-  (s : composition_series im)
+  (s : composition_series X)
   (x : X)
-  (hlt : ∀ y ∈ s, y < x)
-  (hsat : Ico s.top x = {s.top}) :
-  (insert s x hlt hsat).top = x :=
+  (hsat : is_maximal s.top x) :
+  (insert s x hsat).top = x :=
 fin.snoc_last _ _
 
 @[simp] lemma insert_last
-  (s : composition_series im)
+  (s : composition_series X)
   (x : X)
-  (hlt : ∀ y ∈ s, y < x)
-  (hsat : Ico s.top x = {s.top}) :
-  insert s x hlt hsat (fin.last _) = x :=
+  (hsat : is_maximal s.top x) :
+  insert s x hsat (fin.last _) = x :=
 fin.snoc_last _ _
 
 @[simp] lemma insert_cast_succ
-  (s : composition_series im)
+  (s : composition_series X)
   (x : X)
-  (hlt : ∀ y ∈ s, y < x)
-  (hsat : Ico s.top x = {s.top}) (i : fin (s.length + 1)) :
-  insert s x hlt hsat (i.cast_succ) = s i :=
+  (hsat : is_maximal s.top x) (i : fin (s.length + 1)) :
+  insert s x hsat (i.cast_succ) = s i :=
 fin.snoc_cast_succ _ _ _
 
+@[simp] lemma bot_insert
+  (s : composition_series X)
+  (x : X)
+  (hsat : is_maximal s.top x) :
+  (insert s x hsat).bot = s.bot :=
+by rw [bot, bot, ← fin.cast_succ_zero, insert_cast_succ]
+
 lemma mem_insert
-  {s : composition_series im}
+  {s : composition_series X}
   {x y: X}
-  {hlt : ∀ y ∈ s, y < x}
-  {hsat : Ico s.top x = {s.top}} :
-  y ∈ insert s x hlt hsat ↔ y ∈ s ∨ y = x :=
+  {hsat : is_maximal s.top x} :
+  y ∈ insert s x hsat ↔ y ∈ s ∨ y = x :=
 begin
   simp only [insert, mem_def],
   split,
@@ -397,62 +419,67 @@ begin
     { use (fin.last _), simp } }
 end
 
-lemma insert_erase_top
-  {s : composition_series im}
+lemma eq_insert_erase_top
+  {s : composition_series X}
   (h : 0 < s.length) :
   s = insert (erase_top s) s.top
-    (λ y, lt_top_of_mem_erase_top h)
-    (Ico_erase_top_top h) :=
+    (is_maximal_erase_top_top h) :=
 begin
   ext x,
   simp [mem_insert, mem_erase_top h],
   by_cases h : x = s.top; simp [*, s.top_mem]
 end
 
+@[simp] lemma insert_erase_top_top {s : composition_series X}
+  (h : is_maximal s.erase_top.top s.top) :
+  s.erase_top.insert s.top h = s :=
+have h : 0 < s.length,
+  from nat.pos_of_ne_zero begin
+    assume hs,
+    refine ne_of_gt (lt_of_is_maximal h) _,
+    simp [top, fin.ext_iff, hs]
+  end,
+(eq_insert_erase_top h).symm
 
-variables (r : (X × X) → (X × X) → Prop)
-
-def equivalence (s₁ s₂ : composition_series im) : Type* :=
-{ f : fin s₁.length ≃ fin s₂.length //
+def equivalent (s₁ s₂ : composition_series X) : Prop :=
+∃ f : fin s₁.length ≃ fin s₂.length,
   ∀ i : fin s₁.length,
-    r (s₁ i.cast_succ, s₁ i.succ)
-    (s₂ (f i).cast_succ, s₂ (f i).succ) }
+    isom (s₁ i.cast_succ, s₁ i.succ)
+    (s₂ (f i).cast_succ, s₂ (f i).succ)
 
-namespace equivalence
+namespace equivalent
 
-variables [is_equiv _ r]
+@[refl] lemma refl (s : composition_series X) : equivalent s s :=
+⟨equiv.refl _, λ _, isom_refl _⟩
 
-@[refl] def refl (s : composition_series im) : equivalence r s s :=
-⟨equiv.refl _, λ _, is_refl.reflexive _⟩
+@[symm] lemma symm {s₁ s₂ : composition_series X} (h : equivalent s₁ s₂) :
+  equivalent s₂ s₁ :=
+⟨h.some.symm, λ i, isom_symm (by simpa using h.some_spec (h.some.symm i))⟩
 
-@[symm] def symm {s₁ s₂ : composition_series im} (h : equivalence r s₁ s₂) :
-  equivalence r s₂ s₁ :=
-⟨h.1.symm, λ i, is_symm.symm _ _ (by simpa using h.2 (h.1.symm i))⟩
-
-@[trans] def trans {s₁ s₂ s₃ : composition_series im}
-  (h₁ : equivalence r s₁ s₂)
-  (h₂ : equivalence r s₂ s₃) :
-  equivalence r s₁ s₃ :=
-⟨h₁.1.trans h₂.1, λ i, is_trans.trans _ _ _ (h₁.2 i) (h₂.2 (h₁.1 i))⟩
+@[trans] lemma trans {s₁ s₂ s₃ : composition_series X}
+  (h₁ : equivalent s₁ s₂)
+  (h₂ : equivalent s₂ s₃) :
+  equivalent s₁ s₃ :=
+⟨h₁.some.trans h₂.some, λ i, isom_trans (h₁.some_spec i) (h₂.some_spec (h₁.some i))⟩
 
 def append
-  {s₁ s₂ t₁ t₂ : composition_series im}
+  {s₁ s₂ t₁ t₂ : composition_series X}
   (hs : s₁.top = s₂.bot)
   (ht : t₁.top = t₂.bot)
-  (h₁ : equivalence r s₁ t₁)
-  (h₂ : equivalence r s₂ t₂) :
-  equivalence r (append hs) (append ht) :=
+  (h₁ : equivalent s₁ t₁)
+  (h₂ : equivalent s₂ t₂) :
+  equivalent (append hs) (append ht) :=
 let e : fin (s₁.length + s₂.length) ≃ fin (t₁.length + t₂.length) :=
   calc fin (s₁.length + s₂.length) ≃ fin s₁.length ⊕ fin s₂.length : fin_sum_fin_equiv.symm
-  ... ≃ fin t₁.length ⊕ fin t₂.length : equiv.sum_congr h₁.1 h₂.1
+  ... ≃ fin t₁.length ⊕ fin t₂.length : equiv.sum_congr h₁.some h₂.some
   ... ≃ fin (t₁.length + t₂.length) : fin_sum_fin_equiv in
 ⟨e, begin
   assume i,
   refine fin.add_cases _ _ i,
   { assume i,
-    simpa [top, bot] using h₁.2 i },
+    simpa [top, bot] using h₁.some_spec i },
   { assume i,
-    simpa [top, bot] using h₂.2 i }
+    simpa [top, bot] using h₂.some_spec i }
 end⟩
 
 lemma fin.succ_cast_succ {n : ℕ} (i : fin n) :
@@ -460,24 +487,22 @@ lemma fin.succ_cast_succ {n : ℕ} (i : fin n) :
 fin.ext (by simp)
 
 protected lemma insert
-  {s₁ s₂ : composition_series im}
+  {s₁ s₂ : composition_series X}
   {x₁ x₂ : X}
-  {hlt₁ : ∀ y ∈ s₁, y < x₁}
-  {hlt₂ : ∀ y ∈ s₂, y < x₂}
-  {hsat₁ : Ico s₁.top x₁ = {s₁.top}}
-  {hsat₂ : Ico s₂.top x₂ = {s₂.top}}
-  (hequiv : equivalence r s₁ s₂)
-  (htop : r (s₁.top, x₁) (s₂.top, x₂)) :
-  equivalence r (s₁.insert x₁ hlt₁ hsat₁) (s₂.insert x₂ hlt₂ hsat₂) :=
+  {hsat₁ : is_maximal s₁.top x₁}
+  {hsat₂ : is_maximal s₂.top x₂}
+  (hequiv : equivalent s₁ s₂)
+  (htop : isom (s₁.top, x₁) (s₂.top, x₂)) :
+  equivalent (s₁.insert x₁ hsat₁) (s₂.insert x₂ hsat₂) :=
 let e : fin s₁.length.succ ≃ fin s₂.length.succ :=
   calc fin (s₁.length + 1) ≃ option (fin s₁.length) : fin_succ_equiv_last
-  ... ≃ option (fin s₂.length) : functor.map_equiv option hequiv.1
+  ... ≃ option (fin s₂.length) : functor.map_equiv option hequiv.some
   ... ≃ fin (s₂.length + 1) : fin_succ_equiv_last.symm in
 ⟨e,  λ i, begin
   refine fin.last_cases _ _ i,
   { simpa [top] using htop },
   { assume i,
-    simpa [fin.succ_cast_succ] using hequiv.2 i }
+    simpa [fin.succ_cast_succ] using hequiv.some_spec i }
 end⟩
 
 variables {α β : Type*} (e : α ≃ β)
@@ -527,24 +552,20 @@ def option_option_equiv_swap :
   (option_option_equiv_swap e).symm (some a) = some (e.symm a) := rfl
 
 lemma insert_insert_swap
-  {s₁ s₂ : composition_series im}
+  {s₁ s₂ : composition_series X}
   {x₁ x₂ y₁ y₂ : X}
-  {hlt₁ : ∀ y ∈ s₁, y < x₁}
-  {hlt₂ : ∀ y ∈ s₂, y < x₂}
-  {hsat₁ : Ico s₁.top x₁ = {s₁.top}}
-  {hsat₂ : Ico s₂.top x₂ = {s₂.top}}
-  {hlty₁ : ∀ y ∈ insert s₁ x₁ hlt₁ hsat₁, y < y₁}
-  {hlty₂ : ∀ y ∈ insert s₂ x₂ hlt₂ hsat₂, y < y₂}
-  {hsaty₁ : Ico (insert s₁ x₁ hlt₁ hsat₁).top y₁ = {(insert s₁ x₁ hlt₁ hsat₁).top}}
-  {hsaty₂ : Ico (insert s₂ x₂ hlt₂ hsat₂).top y₂ = {(insert s₂ x₂ hlt₂ hsat₂).top}}
-  (hequiv : equivalence r s₁ s₂)
-  (hr₁ : r (s₁.top, x₁) (x₂, y₂))
-  (hr₂ : r (x₁, y₁) (s₂.top, x₂)) :
-  equivalence r
-    (insert (insert s₁ x₁ hlt₁ hsat₁) y₁ hlty₁ hsaty₁)
-    (insert (insert s₂ x₂ hlt₂ hsat₂) y₂ hlty₂ hsaty₂) :=
+  {hsat₁ : is_maximal s₁.top x₁}
+  {hsat₂ : is_maximal s₂.top x₂}
+  {hsaty₁ : is_maximal (insert s₁ x₁ hsat₁).top y₁}
+  {hsaty₂ : is_maximal (insert s₂ x₂ hsat₂).top y₂}
+  (hequiv : equivalent s₁ s₂)
+  (hr₁ : isom (s₁.top, x₁) (x₂, y₂))
+  (hr₂ : isom (x₁, y₁) (s₂.top, x₂)) :
+  equivalent
+    (insert (insert s₁ x₁ hsat₁) y₁ hsaty₁)
+    (insert (insert s₂ x₂ hsat₂) y₂ hsaty₂) :=
 let e : fin (s₁.length + 1 + 1) ≃ fin (s₂.length + 1 + 1) :=
-swap_top_two_fin hequiv.1 in
+swap_top_two_fin hequiv.some in
 ⟨e, begin
   intro i,
   dsimp only [e],
@@ -562,62 +583,98 @@ swap_top_two_fin hequiv.1 in
         insert_cast_succ, insert_cast_succ, fin.succ_cast_succ, insert_cast_succ,
         fin.succ_cast_succ, insert_cast_succ, fin.succ_cast_succ, insert_cast_succ,
         fin.succ_cast_succ, insert_cast_succ],
-      exact hequiv.2 i } }
+      exact hequiv.some_spec i } }
 end⟩
 
-end equivalence
+lemma length_eq {s₁ s₂ : composition_series X} (h : equivalent s₁ s₂) :
+  s₁.length = s₂.length :=
+by simpa using fintype.card_congr h.some
 
+end equivalent
 
-  -- (second_iso : ∀ h k, r (h ⊔ k, k) (h, h ⊓ k))
---   -- (hIco : ∀ g h k : X, Ico h g = {h} → Ico k g = {k} → Ico (h ⊓ k) h = {h ⊓ k}) Not right. Need h ≠ k
-
-lemma length_pos_of_length_pos_of_bot_eq_bot_of_top_eq_top
-  {s₁ s₂ : composition_series im}
-  (hb : s₁.bot = s₂.bot) (ht : s₁.top = s₂.top) :
-  0 < s₁.length →  0 < s₂.length :=
-not_imp_not.1 begin
-  simp only [pos_iff_ne_zero, ne.def, not_iff_not, not_not],
-  assume hs₂,
-  have : s₂.bot = s₂.top,
-    from congr_arg s₂ (fin.ext (by simp [hs₂])),
-  have : (fin.last s₁.length) = (0 : fin s₁.length.succ),
-    from s₁.injective (hb.trans (this.trans ht.symm)).symm,
+lemma length_eq_zero_of_bot_eq_bot_of_top_eq_top_of_length_eq_zero
+  {s₁ s₂ : composition_series X}
+  (hb : s₁.bot = s₂.bot) (ht : s₁.top = s₂.top)
+  (hs₁ : s₁.length = 0) : s₂.length = 0 :=
+begin
+  have : s₁.bot = s₁.top,
+    from congr_arg s₁ (fin.ext (by simp [hs₁])),
+  have : (fin.last s₂.length) = (0 : fin s₂.length.succ),
+    from s₂.injective (hb.symm.trans (this.trans ht)).symm,
   simpa [fin.ext_iff]
 end
--- Maybe a series is just a set?
-theorem jordan_hoelder [is_equiv _ r] (s₁ s₂ : composition_series im)
+
+lemma length_pos_of_bot_eq_bot_of_top_eq_top_of_length_pos
+  {s₁ s₂ : composition_series X}
   (hb : s₁.bot = s₂.bot) (ht : s₁.top = s₂.top) :
-  equivalence r s₁ s₂ :=
-begin
-  induction hle : s₁.length with n ih generalizing s₁ s₂,
-  { admit
-    --  haveI hs : subsingleton X,
-    -- { rw [subsingleton_iff_length_eq_zero, hl] },
-    -- have : s₁.length = s₂.length,
-    -- { rw [hl, eq_comm, ← subsingleton_iff_length_eq_zero,
-    --     s₁.subsingleton_iff_length_eq_zero, hl] },
-    -- use this,
-    -- intros i j hij,
-    -- have : ∀ x : X, x = s₁ i, from λ _, subsingleton.elim _ _,
-    -- rw [this (s₁ j), this (s₂ _), this (s₂ _)],
-    -- exact is_refl.reflexive _
-    },
-  { have h0₁ : 0 < s₁.length, from hle.symm ▸ nat.succ_pos _,
-    have h0₂ : 0 < s₂.length,
-      from length_pos_of_length_pos_of_bot_eq_bot_of_top_eq_top hb ht h0₁,
-    by_cases heq: s₁.erase_top.top = s₂.erase_top.top,
-    { rw [insert_erase_top h0₁, insert_erase_top h0₂],
-      have hr : r (s₁.erase_top.top, s₁.top) (s₂.erase_top.top, s₂.top),
-      { rw [ht, heq], exact is_refl.refl _ },
-      refine equivalence.insert _ _ hr,
-      refine ih _ _ _ _ _,
-      { simp [hb] },
-      { exact heq },
-      { simp [hle] } },
-    { have h0e₁ : 0 < s₁.erase_top.length,
-        from length_pos_of_mem_ne (bot_mem _) (top_mem _) _ }
-
-      }
-
+  0 < s₁.length → 0 < s₂.length :=
+not_imp_not.1 begin
+  simp only [pos_iff_ne_zero, ne.def, not_iff_not, not_not],
+  exact length_eq_zero_of_bot_eq_bot_of_top_eq_top_of_length_eq_zero hb.symm ht.symm
 end
 
+lemma eq_of_bot_eq_bot_of_top_eq_top_of_length_eq_zero
+  {s₁ s₂ : composition_series X}
+  (hb : s₁.bot = s₂.bot) (ht : s₁.top = s₂.top)
+  (hs₁0 : s₁.length = 0) :
+  s₁ = s₂ :=
+have ∀ x, x ∈ s₁ ↔ x = s₁.top,
+  from λ x, ⟨λ hx, forall_mem_eq_of_length_eq_zero hs₁0 hx s₁.top_mem, λ hx, hx.symm ▸ s₁.top_mem⟩,
+have ∀ x, x ∈ s₂ ↔ x = s₂.top,
+  from λ x, ⟨λ hx, forall_mem_eq_of_length_eq_zero
+      (length_eq_zero_of_bot_eq_bot_of_top_eq_top_of_length_eq_zero hb ht hs₁0)
+    hx s₂.top_mem, λ hx, hx.symm ▸ s₂.top_mem⟩,
+by { ext, simp * }
+
+lemma intersection (s : composition_series X) (x : X)
+  (hm : is_maximal x s.top) (hb : s.bot ≤ x) :
+  ∃ t : composition_series X, t.bot = s.bot ∧ t.length + 1 = s.length ∧
+    ∃ htx : t.top = x, equivalent s (insert t s.top (htx.symm ▸ hm)) :=
+begin
+  induction hn : s.length with n ih generalizing s x,
+  { exact (ne_of_gt (lt_of_le_of_lt hb (lt_of_is_maximal hm))
+      (forall_mem_eq_of_length_eq_zero hn s.top_mem s.bot_mem)).elim },
+  { have h0s : 0 < s.length, from hn.symm ▸ nat.succ_pos _,
+    by_cases hetx : s.erase_top.top = x,
+    { use s.erase_top,
+      simp [← hetx, hn] },
+    { have imxs : is_maximal (x ⊓ s.erase_top.top) s.erase_top.top,
+        from is_maximal_inter hm (is_maximal_erase_top_top h0s) (ne.symm hetx),
+      have := ih _ _ imxs (le_inf (by simpa) (le_top s.erase_top.bot_mem)) (by simp [hn]),
+      rcases this with ⟨t, htb, htl, htt, hteqv⟩,
+      have hmtx : is_maximal t.top x,
+      { rw [htt, inf_comm],
+        exact is_maximal_inter (is_maximal_erase_top_top h0s) hm  hetx },
+      use insert t x hmtx,
+      refine ⟨by simp [htb], by simp [htl], by simp, _⟩,
+      have : s.equivalent ((insert t s.erase_top.top (htt.symm ▸ imxs)).insert s.top
+        (by simpa using is_maximal_erase_top_top h0s)),
+      { conv_lhs { rw eq_insert_erase_top h0s },
+        exact equivalent.insert hteqv (by simp) },
+      refine this.trans _,
+      refine equivalent.insert_insert_swap (by refl) _ _,
+      { rw [← sup_eq_of_is_maximal (is_maximal_erase_top_top h0s) hm hetx, htt, inf_comm],
+        exact isom_symm (second_iso s.erase_top.top x) },
+      { rw [← sup_eq_of_is_maximal (is_maximal_erase_top_top h0s) hm hetx, htt, sup_comm],
+        exact second_iso _ _ } } }
+end
+
+theorem jordan_hoelder (s₁ s₂ : composition_series X)
+  (hb : s₁.bot = s₂.bot) (ht : s₁.top = s₂.top) :
+  equivalent s₁ s₂ :=
+begin
+  induction hle : s₁.length with n ih generalizing s₁ s₂,
+  { rw [eq_of_bot_eq_bot_of_top_eq_top_of_length_eq_zero hb ht hle] },
+  { have h0s₂ : 0 < s₂.length,
+      from length_pos_of_bot_eq_bot_of_top_eq_top_of_length_pos hb ht (hle.symm ▸ nat.succ_pos _),
+    rcases intersection s₁ s₂.erase_top.top
+      (ht.symm ▸ is_maximal_erase_top_top h0s₂)
+      (hb.symm ▸ s₂.bot_erase_top ▸ bot_le (top_mem _)) with ⟨t₂, htb₂, htl₂, htt₂, hteq₂⟩,
+    have := ih t₂ s₂.erase_top (by simp [htb₂, ← hb]) htt₂ (nat.succ_inj'.1 (htl₂.trans hle)),
+    refine hteq₂.trans _,
+    conv_rhs { rw [eq_insert_erase_top h0s₂] },
+    simp only [ht],
+    refine equivalent.insert this (by simp [htt₂]) }
+end
+
+end composition_series
